aneris/examples/snapshot_isolation/instantiation/snapshot_isolation_api_implementation.v
@@ -1,0 +1,33 @@
+From aneris.examples.snapshot_isolation
+     Require Import snapshot_isolation_code.
+From aneris.examples.snapshot_isolation.specs
+     Require Import user_params time events resources specs.
+From aneris.examples.snapshot_isolation
+     Require Import snapshot_isolation_code_api.
+From aneris.examples.reliable_communication.prelude Require Import ser_inj.
+
+Section implementation.
+
+  Global Instance KVS_snapshot_isolation_api_implementation :
+          KVS_snapshot_isolation_api :=
+    {|
+      SI_init_server := init_server;
+      SI_start := start;
+      SI_read := read;
+      SI_write := write;
+      SI_commit := commit;
+      SI_run := run;
+      SI_init_client_proxy := init_client_proxy;
+    |}.
+
+  Context `{!anerisG Mdl Σ, !User_params, !KVS_time}.
+
+  Context (KVS_ser_inj : ser_is_injective KVS_serialization).
+  Context (KVS_ser_inj_alt : ser_is_injective_alt KVS_serialization).
+
+  Global Instance SI_implementation_init : SI_init.
+  Proof.
+    (* TODO *)
+  Admitted.
+
+End implementation.
